thys/Pi_Calculus/Pi_Transition.thy
@@ -2,88 +2,8 @@
 the (todo: lazy/eager) pi-calculus transition system
  *)
 theory Pi_Transition
-imports Pi  "../Instantiation_Infrastructure/Curry_LFP" 
-"../Generic_Barendregt_Enhanced_Rule_Induction"
+imports Commitment 
 begin
-
-ML \<open>
-Multithreading.parallel_proofs := 4
-\<close>
-
-local_setup \<open>fn lthy =>
-let
-  val name1 = "commit_internal"
-  val name2 = "commit"
-  val T1 = @{typ "'var term"}
-  val T2 = @{typ "'var * 'var * 'var term +'var * 'var * 'var term + 'var * 'bvar * 'brec"}
-  val Xs = map dest_TFree []
-  val resBs = map dest_TFree [@{typ 'var}, @{typ 'bvar}, @{typ 'brec}, @{typ 'rec}]
-  val rel = [[0]]
-
-  fun flatten_tyargs Ass = subtract (op =) Xs (filter (fn T => exists (fn Ts => member (op =) Ts T) Ass) resBs) @ Xs;
-  val qualify1 = Binding.prefix_name (name1 ^ "_pre_")
-  val qualify2 = Binding.prefix_name (name2 ^ "_pre_")
-
-  (* Step 1: Create pre-MRBNF *)
-  val ((mrbnf1, tys1), (accum, lthy)) = MRBNF_Comp.mrbnf_of_typ true MRBNF_Def.Smart_Inline qualify1 flatten_tyargs Xs []
-    [(dest_TFree @{typ 'var}, MRBNF_Def.Free_Var), (dest_TFree @{typ 'bvar}, MRBNF_Def.Bound_Var)] T1
-    ((MRBNF_Comp.empty_comp_cache, MRBNF_Comp.empty_unfolds), lthy)
-  val ((mrbnf2, tys2), (accum, lthy)) = MRBNF_Comp.mrbnf_of_typ true MRBNF_Def.Smart_Inline qualify2 flatten_tyargs Xs []
-    [(dest_TFree @{typ 'var}, MRBNF_Def.Free_Var), (dest_TFree @{typ 'bvar}, MRBNF_Def.Bound_Var)] T2
-    (accum, lthy);
-
-  val (tys, _, (mrbnfs as [mrbnf1, mrbnf2], (accum, lthy))) =
-      MRBNF_Comp.normalize_mrbnfs (K I) [] (map (map dest_TFree) [snd tys1, snd tys2])
-      [] (K (resBs @ Xs)) NONE [mrbnf1, mrbnf2] (accum, lthy);
-
-  (* Step 2: Seal the pre-MRBNF with a typedef *)
-  val ((mrbnf1, (Ds, info)), lthy) = MRBNF_Comp.seal_mrbnf I (snd accum) (Binding.name (name1 ^ "_pre")) true (fst tys1) [] mrbnf1 lthy
-  val ((mrbnf2, (Ds, info)), lthy) = MRBNF_Comp.seal_mrbnf I (snd accum) (Binding.name (name2 ^ "_pre")) true (fst tys2) [] mrbnf2 lthy
-
-  (* Step 3: Register the pre-MRBNF as a BNF in its live variables *)
-  val (bnf1, lthy) = MRBNF_Def.register_mrbnf_as_bnf mrbnf1 lthy
-  val (bnf2, lthy) = MRBNF_Def.register_mrbnf_as_bnf mrbnf2 lthy
-
-  (* Step 4: Create fixpoint of pre-MRBNF *)
-  val (res, lthy) = MRBNF_FP.construct_binder_fp MRBNF_Util.Least_FP [
-    ((name1, mrbnf1), 1), ((name2, mrbnf2), 1)
-  ] rel lthy;
-in lthy end
-\<close>
-print_theorems
-
-definition Finp :: "'a::{var_commit_pre,var_commit_internal_pre} \<Rightarrow> 'a \<Rightarrow> 'a term \<Rightarrow> 'a commit" where
-  "Finp x y t \<equiv> commit_ctor (Abs_commit_pre (Inl (x, y, t)))"
-definition Fout :: "'a::{var_commit_pre,var_commit_internal_pre} \<Rightarrow> 'a \<Rightarrow> 'a term \<Rightarrow> 'a commit" where
-  "Fout x y t \<equiv> commit_ctor (Abs_commit_pre (Inr (Inl (x, y, t))))"
-definition Bout :: "'a::{var_commit_pre,var_commit_internal_pre} \<Rightarrow> 'a \<Rightarrow> 'a term \<Rightarrow> 'a commit" where
-  "Bout x y t \<equiv> commit_ctor (Abs_commit_pre (Inr (Inr (x, y, commit_internal_ctor (Abs_commit_internal_pre t)))))"
-
-lemma FFVars_commit_simps[simp]:
-  "FFVars_commit (Finp x y t) = {x, y} \<union> FFVars_term t"
-  "FFVars_commit (Fout x y t) = {x, y} \<union> FFVars_term t"
-  "FFVars_commit (Bout x y t) = {x} \<union> (FFVars_term t - {y})"
-  apply (unfold Bout_def Finp_def Fout_def)
-  apply (rule trans)
-     apply (rule commit_internal.FFVars_cctors)
-    defer
-    apply (rule trans, rule commit_internal.FFVars_cctors)
-    defer
-    apply (rule trans, rule commit_internal.FFVars_cctors)
-  apply (unfold set1_commit_pre_def comp_def Abs_commit_pre_inverse[OF UNIV_I] map_prod_simp
-    UN_empty UN_empty2 prod_set_simps set3_commit_pre_def cSup_singleton Un_empty_left Un_empty_right
-    Sup_empty set2_commit_pre_def set4_commit_pre_def UN_single map_sum.simps sum_set_simps
-  )
-    apply (rule arg_cong2[OF refl, of _ _ "(\<union>)"])
-apply (rule arg_cong2[OF _ refl, of _ _ minus])
-  apply (rule trans)
-   apply (rule commit_internal.FFVars_cctors)
-  apply (unfold set1_commit_internal_pre_def comp_def Abs_commit_internal_pre_inverse[OF UNIV_I] map_prod_simp prod_set_simps
-    UN_empty cSup_singleton Un_empty_left Un_empty_right set3_commit_internal_pre_def empty_Diff
-    set4_commit_internal_pre_def
-  )
-    apply auto
-  done
 
 (* INSTANTIATING THE ABSTRACT SETTING: *)
 
@@ -93,18 +13,16 @@ print_locales
 interpretation Small where dummy = "undefined :: var" 
 apply standard
 by (simp_all add: infinite_var regularCard_var)  
-
-
-abbreviation "usub P y x \<equiv> vvsubst (id(x:=y)) P"
  
 
 (* AN EXAMPLE INDUCTIVE DEFINITION *)
 (* (a reduced form of) small trans semantics *) 
-find_theorems vvsubst
-inductive trans :: "trm \<Rightarrow> trm \<Rightarrow> bool" where
-Inp: "trans (Inp a x P) (usub P y x)"
+inductive trans :: "trm \<Rightarrow> cmt \<Rightarrow> bool" where
+Inp: "x \<notin> {a,u} \<Longrightarrow> trans (Inp a x P) (Finp a u (usub P u x))"
 |
-Out: "trans (Out a x P) (usub P y x)"
+Out: "trans (Out a x P) (Fout a x P)"
+|
+Tau: "trans P (Tau P)"
 
 
 
