thys/Pi_Calculus/Commitment.thy
@@ -1,0 +1,222 @@
+theory Commitment
+imports Pi  "../Instantiation_Infrastructure/Curry_LFP" 
+"../Generic_Barendregt_Enhanced_Rule_Induction"
+begin
+
+ML \<open>
+Multithreading.parallel_proofs := 4
+\<close>
+
+local_setup \<open>fn lthy =>
+let
+  val name1 = "commit_internal"
+  val name2 = "commit"
+  val T1 = @{typ "'var term"}
+  val T2 = @{typ "'var * 'var * 'var term +'var * 'var * 'var term + 'var * 'bvar * 'brec + 'var term"}
+  val Xs = map dest_TFree []
+  val resBs = map dest_TFree [@{typ 'var}, @{typ 'bvar}, @{typ 'brec}, @{typ 'rec}]
+  val rel = [[0]]
+
+  fun flatten_tyargs Ass = subtract (op =) Xs (filter (fn T => exists (fn Ts => member (op =) Ts T) Ass) resBs) @ Xs;
+  val qualify1 = Binding.prefix_name (name1 ^ "_pre_")
+  val qualify2 = Binding.prefix_name (name2 ^ "_pre_")
+
+  (* Step 1: Create pre-MRBNF *)
+  val ((mrbnf1, tys1), (accum, lthy)) = MRBNF_Comp.mrbnf_of_typ true MRBNF_Def.Smart_Inline qualify1 flatten_tyargs Xs []
+    [(dest_TFree @{typ 'var}, MRBNF_Def.Free_Var), (dest_TFree @{typ 'bvar}, MRBNF_Def.Bound_Var)] T1
+    ((MRBNF_Comp.empty_comp_cache, MRBNF_Comp.empty_unfolds), lthy)
+  val ((mrbnf2, tys2), (accum, lthy)) = MRBNF_Comp.mrbnf_of_typ true MRBNF_Def.Smart_Inline qualify2 flatten_tyargs Xs []
+    [(dest_TFree @{typ 'var}, MRBNF_Def.Free_Var), (dest_TFree @{typ 'bvar}, MRBNF_Def.Bound_Var)] T2
+    (accum, lthy);
+
+  val (tys, _, (mrbnfs as [mrbnf1, mrbnf2], (accum, lthy))) =
+      MRBNF_Comp.normalize_mrbnfs (K I) [] (map (map dest_TFree) [snd tys1, snd tys2])
+      [] (K (resBs @ Xs)) NONE [mrbnf1, mrbnf2] (accum, lthy);
+
+  (* Step 2: Seal the pre-MRBNF with a typedef *)
+  val ((mrbnf1, (Ds, info)), lthy) = MRBNF_Comp.seal_mrbnf I (snd accum) (Binding.name (name1 ^ "_pre")) true (fst tys1) [] mrbnf1 lthy
+  val ((mrbnf2, (Ds, info)), lthy) = MRBNF_Comp.seal_mrbnf I (snd accum) (Binding.name (name2 ^ "_pre")) true (fst tys2) [] mrbnf2 lthy
+
+  (* Step 3: Register the pre-MRBNF as a BNF in its live variables *)
+  val (bnf1, lthy) = MRBNF_Def.register_mrbnf_as_bnf mrbnf1 lthy
+  val (bnf2, lthy) = MRBNF_Def.register_mrbnf_as_bnf mrbnf2 lthy
+
+  (* Step 4: Create fixpoint of pre-MRBNF *)
+  val (res, lthy) = MRBNF_FP.construct_binder_fp MRBNF_Util.Least_FP [
+    ((name1, mrbnf1), 1), ((name2, mrbnf2), 1)
+  ] rel lthy;
+in lthy end
+\<close>
+print_theorems
+
+
+(* Monomorphization: *)
+type_synonym cmt = "var commit"
+instance var :: var_commit_pre by standard
+instance var :: var_commit_internal_pre by standard
+
+definition Finp :: "var \<Rightarrow> var \<Rightarrow> trm \<Rightarrow> cmt" where
+  "Finp x y t \<equiv> commit_ctor (Abs_commit_pre (Inl (x, y, t)))"
+definition Fout :: "var \<Rightarrow> var \<Rightarrow> trm \<Rightarrow> cmt" where
+  "Fout x y t \<equiv> commit_ctor (Abs_commit_pre (Inr (Inl (x, y, t))))"
+definition Bout :: "var \<Rightarrow> var \<Rightarrow> trm \<Rightarrow> cmt" where
+  "Bout x y t \<equiv> commit_ctor (Abs_commit_pre (Inr (Inr (Inl (x, y, commit_internal_ctor (Abs_commit_internal_pre t))))))"
+definition Tau :: "trm \<Rightarrow> cmt" where
+  "Tau t \<equiv> commit_ctor (Abs_commit_pre (Inr (Inr (Inr t))))"
+
+lemmas toUnfold = set1_commit_internal_pre_def
+  UN_empty UN_empty2 UN_single Un_empty_left Un_empty_right
+  comp_def empty_Diff
+  map_prod_simp prod_set_simps
+  map_sum.simps sum_set_simps prod_set_simps 
+  Sup_empty cSup_singleton 
+  (* *)
+  Abs_commit_pre_inverse[OF UNIV_I]
+  set1_commit_pre_def set2_commit_pre_def set4_commit_pre_def set3_commit_pre_def  
+  Abs_commit_internal_pre_inverse[OF UNIV_I]  
+  set1_commit_internal_pre_def set2_commit_internal_pre_def
+  set3_commit_internal_pre_def set4_commit_internal_pre_def
+
+lemma FFVars_commit_simps[simp]: 
+  "FFVars_commit (Finp x y t) = {x, y} \<union> FFVars t"
+  "FFVars_commit (Fout x y t) = {x, y} \<union> FFVars t"
+  "FFVars_commit (Bout x y t) = {x} \<union> (FFVars t - {y})"
+  "FFVars_commit (Tau t) = FFVars t"
+  apply (unfold Bout_def Finp_def Fout_def Tau_def)
+  apply (rule trans)
+     apply (rule commit_internal.FFVars_cctors)
+    defer
+    apply (rule trans, rule commit_internal.FFVars_cctors)
+    defer
+    apply (rule trans, rule commit_internal.FFVars_cctors)
+  apply (unfold toUnfold)
+    apply (rule arg_cong2[OF refl, of _ _ "(\<union>)"])
+apply (rule arg_cong2[OF _ refl, of _ _ minus])
+  apply (rule trans)
+   apply (rule commit_internal.FFVars_cctors)
+  apply (unfold toUnfold)
+    apply auto 
+  subgoal
+    unfolding commit_internal.FFVars_cctors(2) 
+    apply (unfold toUnfold) by auto
+  subgoal
+    unfolding commit_internal.FFVars_cctors(2) 
+    apply (unfold toUnfold) by auto
+  done
+
+lemmas commit_pre.map_id0[simp]
+lemmas commit_pre_map_cong_id = commit_pre.map_cong[of _ _ "id::var\<Rightarrow>var" "id::var\<Rightarrow>var" _ _ _ id _ id, simplified] 
+
+lemma map_commit_pre_Inl_aux: "bij f \<Longrightarrow> |supp f| <o |UNIV::var set| \<Longrightarrow> 
+ map_commit_pre (id::var\<Rightarrow>var) (f::var\<Rightarrow>var) (rrename_commit_internal f) id (Abs_commit_pre (Inl (x, y, P))) = 
+ Abs_commit_pre (Inl (x, y, P))"
+apply(rule commit_pre_map_cong_id) unfolding toUnfold by auto 
+
+lemma map_commit_pre_Inr_Inl_aux: "bij f \<Longrightarrow> |supp f| <o |UNIV::var set| \<Longrightarrow> 
+ map_commit_pre (id::var\<Rightarrow>var) (f::var\<Rightarrow>var) (rrename_commit_internal f) id (Abs_commit_pre (Inr (Inl (x, y, P)))) = 
+ Abs_commit_pre (Inr (Inl (x, y, P)))"
+apply(rule commit_pre_map_cong_id) unfolding toUnfold by auto
+
+lemma map_commit_pre_Inr_Inr_Inl_aux: "bij f \<Longrightarrow> |supp f| <o |UNIV::var set| \<Longrightarrow> 
+ map_commit_pre id f (rrename_commit_internal f) id
+          (Abs_commit_pre (Inr (Inr (Inl (x, y, commit_internal_ctor (Abs_commit_internal_pre P)))))) = 
+ Abs_commit_pre (Inr (Inr (Inl (x, f y, commit_internal_ctor (Abs_commit_internal_pre (rrename f P))))))"
+unfolding map_commit_pre_def toUnfold apply auto 
+unfolding commit_internal.rrename_cctors(1)
+apply(subst commit_internal.rrename_cctors(1)) apply auto
+  subgoal sorry (* AtoJ: what UNIV is this? *)
+  subgoal unfolding map_commit_internal_pre_def apply (auto simp: toUnfold) 
+    by (simp add: \<open>\<lbrakk>bij f; |supp f| <o |UNIV|\<rbrakk> \<Longrightarrow> |supp f| <o |UNIV|\<close>) .
+
+
+lemma map_commit_pre_Inr_Inr_Inr_aux: "bij f \<Longrightarrow> |supp f| <o |UNIV::var set| \<Longrightarrow> 
+ map_commit_pre (id::var\<Rightarrow>var) (f::var\<Rightarrow>var) (rrename_commit_internal f) id (Abs_commit_pre (Inr (Inr (Inr P)))) = 
+ Abs_commit_pre (Inr (Inr (Inr P)))"
+apply(rule commit_pre_map_cong_id) unfolding toUnfold by auto
+
+lemma Abs_commit_pre_inj[simp]: "Abs_commit_pre k = Abs_commit_pre k' \<longleftrightarrow> k = k'"
+by (metis toUnfold(22))
+
+lemma Abs_commit_internal_pre_inj[simp]: "Abs_commit_internal_pre k = Abs_commit_internal_pre k' \<longleftrightarrow> k = k'"
+by (metis toUnfold(27))
+
+lemma Finp_inj[simp]: "Finp x y P = Finp x' y' P' \<longleftrightarrow> x = x' \<and> y = y' \<and> P = P'"
+unfolding Finp_def unfolding commit_internal.TT_injects0 apply simp
+unfolding toUnfold apply auto
+  subgoal for f apply(subst (asm) map_commit_pre_Inl_aux) by auto 
+  subgoal for f apply(subst (asm) map_commit_pre_Inl_aux) by auto 
+  subgoal for f apply(subst (asm) map_commit_pre_Inl_aux) by auto 
+  subgoal apply(rule exI[of _ id]) apply(subst map_commit_pre_Inl_aux) by auto .
+
+lemma Fout_inj[simp]: "Fout x y P = Fout x' y' P' \<longleftrightarrow> x = x' \<and> y = y' \<and> P = P'"
+unfolding Fout_def unfolding commit_internal.TT_injects0 apply simp
+unfolding toUnfold apply auto
+  subgoal for f apply(subst (asm) map_commit_pre_Inr_Inl_aux) by auto 
+  subgoal for f apply(subst (asm) map_commit_pre_Inr_Inl_aux) by auto 
+  subgoal for f apply(subst (asm) map_commit_pre_Inr_Inl_aux) by auto 
+  subgoal apply(rule exI[of _ id]) apply(subst map_commit_pre_Inr_Inl_aux) by auto .
+
+lemma Bout_inj[simp]: "Bout x y P = Bout x' y' P' \<longleftrightarrow> x = x' \<and> ((y' \<notin> FFVars P \<or> y' = y) \<and> P' = swap P y y')"
+unfolding Bout_def unfolding commit_internal.TT_injects0 apply simp
+unfolding toUnfold apply auto
+  subgoal for f apply(subst (asm) map_commit_pre_Inr_Inr_Inl_aux) by auto 
+  subgoal for f apply(subst (asm) map_commit_pre_Inr_Inr_Inl_aux) 
+  unfolding id_on_def apply auto unfolding commit_internal.FFVars_cctors(1) toUnfold by auto
+  subgoal for f apply(subst (asm) map_commit_pre_Inr_Inr_Inl_aux) 
+  unfolding id_on_def apply auto unfolding commit_internal.FFVars_cctors(1) toUnfold 
+  unfolding commit_internal.TT_injects0(1) id_on_def  
+  unfolding map_commit_internal_pre_def apply (auto simp: toUnfold id_on_def)
+  apply(rule rrename_cong) by auto
+  subgoal apply(rule exI[of _ "(id(y:=y',y':=y))"]) 
+  apply(subst map_commit_pre_Inr_Inr_Inl_aux) apply auto
+  unfolding commit_internal.FFVars_cctors(1) by (auto simp: toUnfold id_on_def) 
+  subgoal apply(rule exI[of _ "(id(y:=y',y':=y))"]) 
+  apply(subst map_commit_pre_Inr_Inr_Inl_aux) apply auto
+  unfolding commit_internal.FFVars_cctors(1) apply (auto simp: toUnfold id_on_def) 
+  by (metis bij_swap supp_swap_bound fun_upd_upd)+ .
+
+lemma Tau_inj[simp]: "Tau P = Tau P' \<longleftrightarrow> P = P'"
+unfolding Tau_def unfolding commit_internal.TT_injects0 apply simp
+unfolding toUnfold apply auto
+  subgoal for f apply(subst (asm) map_commit_pre_Inr_Inr_Inr_aux) by auto  
+  subgoal apply(rule exI[of _ id]) apply(subst map_commit_pre_Inr_Inr_Inr_aux) by auto .
+
+(* *)
+
+lemma Finp_Fout_diff[simp]: "Finp x y P \<noteq> Fout x' y' P'"
+unfolding Finp_def Fout_def  
+by (metis Abs_commit_pre_inj Inl_Inr_False commit_internal.TT_injects0(2) map_commit_pre_Inl_aux)
+
+lemmas Fout_Finp_diff[simp] = Finp_Fout_diff[symmetric]
+
+lemma Finp_Bout_diff[simp]: "Finp x y P \<noteq> Bout x' y' P'"
+unfolding Finp_def Bout_def  
+by (metis Abs_commit_pre_inj Inl_Inr_False commit_internal.TT_injects0(2) map_commit_pre_Inl_aux)
+
+lemmas Bout_Finp_diff[simp] = Finp_Bout_diff[symmetric]
+
+lemma Finp_Tau_diff[simp]: "Finp x y P \<noteq> Tau P'"
+unfolding Finp_def Tau_def  
+by (metis Abs_commit_pre_inj Inl_Inr_False commit_internal.TT_injects0(2) map_commit_pre_Inl_aux)
+
+lemmas Tau_Finp_diff[simp] = Finp_Tau_diff[symmetric]
+
+lemma Fout_Bout_diff[simp]: "Fout x y P \<noteq> Bout x' y' P'"
+unfolding Fout_def Bout_def 
+by (metis Abs_commit_pre_inj Inl_Inr_False commit_internal.TT_injects0(2) map_commit_pre_Inr_Inl_aux sum.inject(2))
+
+lemmas Bout_Fout_diff[simp] = Fout_Bout_diff[symmetric]
+
+lemma Fout_Tau_diff[simp]: "Fout x y P \<noteq> Tau P'"
+unfolding Fout_def Tau_def 
+by (metis Abs_commit_pre_inj Inl_Inr_False commit_internal.TT_injects0(2) map_commit_pre_Inr_Inl_aux sum.inject(2)) 
+
+lemmas Tau_Fout_diff[simp] = Fout_Tau_diff[symmetric]
+
+lemma Bout_Tau_diff[simp]: "Bout x y P \<noteq> Tau P'"
+unfolding Bout_def Tau_def 
+by (smt (verit) Inl_Inr_False Inr_inject commit_internal.TT_injects0(2) map_commit_pre_Inr_Inr_Inl_aux toUnfold(22))
+
+lemmas Tau_Bout_diff[simp] = Bout_Tau_diff[symmetric]
+
+end
